{
 "cells": [
  {
   "cell_type": "markdown",
   "id": "1b2334d5-1d39-42a5-8e84-e00365518396",
   "metadata": {},
   "source": [
    "Pre-Midterm Assignment - Renee Rosary H. Pintor, CIS 1203 Group 1 TTH 10:30 AM - 12:30 PM"
   ]
  },
  {
   "cell_type": "markdown",
   "id": "e1164f52-56dc-459e-aa96-78dd03e11fbb",
   "metadata": {},
   "source": [
    "1. Recall the definition of a rational number, denoted as $\\mathbb{Q}$. Prove that the Euler's number $e = \\sum_{k=0}^\\infty \\frac{1}{k!} \\notin \\mathbb{Q}$. A factorial is defined as $k! = (k)(k-1)(k-2)(k-3)..., \\forall k \\in \\mathbb{Z}^+$, note that $0! = 1$. Furthermore, a sum notation $\\sum_{k=0}^\\infty k = 0+ 1 + 2 + 3 +....+...$\n"
   ]
  },
  {
   "cell_type": "markdown",
   "id": "48390f5a-2327-4008-9d94-4930665a4630",
   "metadata": {},
   "source": [
    "Proof:\n",
    "\n",
    "If e is a rational number, there exist positive integers a and b such that \n",
    "\\begin{equation}\n",
    "    e = \\frac{a}{b}.\n",
    "\\end{equation}\n",
    "Define the number\n",
    "\n",
    "\\begin{equation}\n",
    "    x = b! \\left(e - \\sum_{n=0}^{b} \\frac{1}{n!}\\right).\n",
    "\\end{equation}\n",
    "\n",
    "Use the assumption that \n",
    "\\begin{equation}\n",
    "    e = \\frac{a}{b}\n",
    "\\end{equation} \n",
    "to obtain\n",
    "\n",
    "\\begin{equation}\n",
    "    x = b! \\left(\\frac{a}{b} - \\sum_{n=0}^{b} \\frac{1}{n!}\\right) = a(b-1)! - \\sum_{n=0}^{b} \\frac{b!}{n!}.\n",
    "\\end{equation}\n",
    "\n",
    "The first term is an integer, and every fraction in the sum is actually an integer because \\begin{equation} n \\leq b \\end{equation} for each term. Therefore, under the assumption that e is rational, x is an integer.\n",
    "\n",
    "We now prove that 0 < x < 1. First, to prove that x is strictly positive, we insert the above series representation of e into the definition of x and obtain\n",
    "\n",
    "\\begin{equation}\n",
    "    x = b! \\left(\\sum_{n=0}^\\infty \\frac{1}{n!} - \\sum_{n=0}^{b} \\frac{1}{n!}\\right) = \\sum_{n=b+1}^\\infty \\frac{b!}{n!} > 0,\n",
    "\\end{equation}\n",
    "\n",
    "because all the terms are strictly positive.\n",
    "\n",
    "We now prove that x < 1. For all terms with \\begin{equation} n \\geq b + 1 \\end{equation}, we have the upper estimate\n",
    "\n",
    "\\begin{equation}\n",
    "    \\frac{b!}{n!} = \\frac{1}{(b+1)(b+2)\\cdots(b+(n-b))} \\leq \\frac{1}{(b+1)^{n-b}}.\n",
    "\\end{equation}\n",
    "\n",
    "This inequality is strict for every \\begin{equation} n \\geq b + 2 \\end{equation}. Changing the index of summation to k = n - b and using the formula for the infinite geometric series, we obtain\n",
    "\n",
    "\\begin{equation}\n",
    "    x = \\sum_{n=b+1}^\\infty \\frac{b!}{n!} < \\sum_{n=b+1}^\\infty \\frac{1}{(b+1)^{n-b}} = \\sum_{k=1}^\\infty \\frac{1}{(b+1)^k} = \\frac{1}{b+1} \\left(\\frac{1}{1 - \\frac{1}{b+1}}\\right) = \\frac{1}{b} \\leq 1.\n",
    "\\end{equation}\n",
    "\n",
    "And therefore x < 1.\n",
    "\n",
    "Since there is no integer strictly between 0 and 1, we have reached a contradiction, and so e is irrational, Q.E.D. \n",
    "\n"
   ]
  },
  {
   "cell_type": "markdown",
   "id": "e39ea717-3888-48f3-9c45-a922396ee95a",
   "metadata": {},
   "source": [
    "2. Prove Minkowski's Inequality for sums, $\\forall \\ p>1, (a_k, b_k)>0$:\n",
    "\\begin{gather}\n",
    "\\begin{bmatrix}\n",
    "\\sum_{k=1}^n |a_k + b_k|^p\n",
    "\\end{bmatrix}^\\frac{1}{p}\n",
    "\\leq\n",
    "\\begin{bmatrix}\n",
    "\\sum_{k=1}^n |a_k|^p\n",
    "\\end{bmatrix}^\\frac{1}{p}\n",
    "+\n",
    "\\begin{bmatrix}\n",
    "\\sum_{k=1}^n |b_k|^p\n",
    "\\end{bmatrix}^\\frac{1}{p}\n",
    "\\end{gather}\n"
   ]
  },
  {
   "cell_type": "markdown",
   "id": "c3bbd5f4-ea88-43c6-a3a4-b04a457c7a61",
   "metadata": {},
   "source": [
    "Proof:\n",
    "\n",
    "We start by defining \\begin{aligned} q = \\frac{p}{p - 1} \\end{aligned}. \n",
    "\n",
    "Then:\n",
    "\\begin{aligned} \\frac{1}{p} + \\frac{1}{q} = \\frac{1}{p} + \\frac{p - 1}{p} = 1  \\end{aligned}.\n",
    "\n",
    "It follows that:\n",
    "\\begin{equation}\n",
    "\\begin{split}\n",
    "\\sum_{k=1}^{n}(a_k+b_k)^p & = \\sum_{k=1}^{n} a_k(a_k+b_k)^{p-1} + \\sum_{k=1}^{n} b_k(a_k+b_k)^{p-1} \\\\\n",
    "& \\leq (\\sum_{k=1}^{n} a_k^p)^{1/p} (\\sum_{k=1}^{n} ((a_k+b_k)^{p-1})^q)^{1/q} + (\\sum_{k=1}^{n} b_k^p)^{1/p} (\\sum_{k=1}^{n} ((a_k+b_k)^{p-1})^q)^{1/q} \\quad \\text{(Hölder's Inequality for Sums, twice)} \\\\ \n",
    "& = (\\sum_{k=1}^{n} a_k^p)^{1/p} (\\sum_{k=1}^{n} (a_k+b_k)^p)^{1/q} + (\\sum_{k=1}^{n} b_k^p)^{1/p} (\\sum_{k=1}^{n} (a_k+b_k)^p)^{1/q} \\quad \\text{Power of a Power, and by hypothesis:} \\quad (p-1)q = p\\\\\n",
    "& = ((\\sum_{k=1}^{n} a_k^p)^{1/p} + (\\sum_{k=1}^{n} b_k^p)^{1/p}) (\\sum_{k=1}^{n} (a_k+b_k)^p)^{1/q} \\\\\n",
    "& \\hspace{10mm} \\\\\n",
    "\\Rightarrow \\quad (\\sum_{k=1}^{n} (a_k+b_k)^p)^{1-1/q} & \\leq (\\sum_{k=1}^{n} a_k^p)^{1/p} + (\\sum_{k=1}^{n} b_k^p)^{1/p}  \\quad \\text{(dividing by} \\quad (\\sum_{k=1}^{n} (a_k+b_k)^p)^{1/q}) \\\\\n",
    "& \\Rightarrow \\quad (\\sum_{k=1}^{n} (a_k+b_k)^p)^{1/p} \\leq (\\sum_{k=1}^{n} a_k^p)^{1/p} + (\\sum_{k=1}^{n} b_k^p)^{1/p} \\quad \\text{(as} \\quad 1-\\frac{1}{q} = p) \\\\\n",
    "& \\text{This is equivalent to the given inequality in matrix form:} \\\\\n",
    "& \\begin{bmatrix}\n",
    "\\sum_{k=1}^n |a_k + b_k|^p\n",
    "\\end{bmatrix}^\\frac{1}{p} \\\\\n",
    "& \\leq\n",
    "\\begin{bmatrix}\n",
    "\\sum_{k=1}^n |a_k|^p\n",
    "\\end{bmatrix}^\\frac{1}{p}\n",
    "+\n",
    "\\begin{bmatrix}\n",
    "\\sum_{k=1}^n |b_k|^p\n",
    "\\end{bmatrix}^\\frac{1}{p}\n",
    "\\end{split}\n",
    "\\end{equation}\n",
    "\n",
    "Q.E.D.\n"
   ]
  },
  {
   "cell_type": "markdown",
   "id": "387f74d3-746c-446e-a06f-d3c7b0958d69",
   "metadata": {},
   "source": [
    "3. Prove the triangle inequality $|x+y| \\leq |x| + |y|$, $\\forall (x,y) \\in \\mathbb{R}$"
   ]
  },
  {
   "cell_type": "markdown",
   "id": "fcc7b14e-fc24-46c2-b7eb-19631abc8f4f",
   "metadata": {},
   "source": [
    "Proof that for all $(x,y) \\in \\mathbb{R}$, $|x+y| \\leq |x| + |y|$:\n",
    "\n",
    "The definition of absolute value:\n",
    "\n",
    "\\begin{equation}\n",
    "|x+y| = \\begin{cases} \n",
    "              x+y & \\text{if } x+y \\geq 0 \\\\\n",
    "              -(x+y) & \\text{if } x+y < 0 \n",
    "           \\end{cases}\n",
    "\\end{equation}\n",
    "\n",
    "notice these four inequalities:\n",
    "\\begin{equation}\n",
    "x \\leq |x| \\quad \\text{and} \\quad -x \\leq |x|\n",
    "\\end{equation}\n",
    "\\begin{equation}\n",
    "y \\leq |y| \\quad \\text{and} \\quad -y \\leq |y|\n",
    "\\end{equation}\n",
    "\n",
    "let's start with x+y:\n",
    "\n",
    "since we know that \\begin{equation}x \\leq |x| \\quad \\text{and} \\quad y \\leq |y| \\quad\\end{equation}\n",
    "then\n",
    "\\begin{equation}\n",
    "x + y \\leq |x| + |y|\n",
    "\\end{equation}\n",
    "\n",
    "next is -(a+b):\n",
    "\n",
    "first distribute the negative\n",
    "\\begin{equation}\n",
    "-(x+y) = -x + (-y)\n",
    "\\end{equation}\n",
    "\n",
    "since we know that \\begin{equation}-x \\leq |x| \\quad \\text{and} \\quad -y \\leq |y| \\quad\\end{equation}\n",
    "then\n",
    "\\begin{equation}\n",
    "-x + (-y) \\leq |x| + |y|\n",
    "\\end{equation}\n",
    "\n",
    "By definition |x+y| has to be equal to x+y or -(x+y) and we just showed that \n",
    "\\begin{equation}\n",
    "x + y \\leq |x| + |y|\n",
    "\\end{equation}\n",
    "and \n",
    "\\begin{equation}\n",
    "-x + (-y) \\leq |x| + |y|\n",
    "\\end{equation}\n",
    "\n",
    "thus we know for sure that\n",
    "$|x+y| \\leq |x| + |y|$\n",
    "\n",
    "Q.E.D.\n",
    "\n"
   ]
  },
  {
   "cell_type": "markdown",
   "id": "51d9ec54-10bb-4e1e-9915-871676297d3a",
   "metadata": {},
   "source": [
    "4. Prove Sedrakayan's Lemma $\\forall u_i, v_i \\in \\mathbb{R}^+$:\n",
    "\\begin{gather}\n",
    "\\frac{(\\sum_{i=1}^n u_i)^2}{\\sum_{i=1}^n v_i} \\leq \\sum_{i=1}^n \\frac{(u_i)^2}{v_i}\n",
    "\\end{gather}\n"
   ]
  },
  {
   "cell_type": "markdown",
   "id": "7e8c5df0-707b-4aca-9d98-f0065b232321",
   "metadata": {},
   "source": [
    "We want to prove that for all non-negative real numbers $u_i, v_i \\in \\mathbb{R}^+$:\n",
    "\n",
    "$$\\frac{(\\sum_{i=1}^n u_i)^2}{\\sum_{i=1}^n v_i} \\leq \\sum_{i=1}^n \\frac{(u_i)^2}{v_i}$$\n",
    "\n",
    "Proof:\n",
    "\n",
    "1. Rearrangement Inequality:\n",
    "\n",
    "   We can utilize the Rearrangement Inequality which states that for any non-negative real numbers $a_1, a_2, \\ldots, a_n$ and $b_1, b_2, \\ldots, b_n$ such that $a_1 \\ge a_2 \\ge \\ldots \\ge a_n$ and $b_1 \\le b_2 \\le \\ldots \\le b_n$, the following holds:\n",
    "\n",
    "   $$a_1 b_1 + a_2 b_2 + \\ldots + a_n b_n \\ge a_1 b_n + a_2 b_{n-1} + \\ldots + a_n b_1$$\n",
    "\n",
    "2. Applying the Inequality:\n",
    "\n",
    "   Let's define $a_i = u_i^2$ and $b_i = v_i$. Since $u_i, v_i \\in \\mathbb{R}^+$, then $a_i$ and $b_i$ are also non-negative real numbers. The Rearrangement Inequality can be applied as follows, but note that the order of $v_i$ must be preserved on both sides:\n",
    "\n",
    "   $$a_1 b_1 + a_2 b_2 + \\ldots + a_n b_n \\leq a_1 b_n + a_2 b_{n-1} + \\ldots + a_n b_1$$\n",
    "\n",
    "   Substituting $a_i = u_i^2$ and $b_i = v_i$, we get:\n",
    "\n",
    "   $$\\sum_{i=1}^n (u_i^2) \\cdot v_i \\leq \\sum_{i=1}^n u_i^2 \\cdot v_1$$\n",
    "\n",
    "   This can be rewritten as:\n",
    "\n",
    "   $$\\sum_{i=1}^n u_i^2 \\cdot \\frac{1}{v_i} \\leq \\frac{(\\sum_{i=1}^n u_i)^2}{v_1}$$\n",
    "\n",
    "3. Conclusion:\n",
    "\n",
    "   Notice that after applying the Rearrangement Inequality, we have $\\frac{(\\sum_{i=1}^n u_i)^2}{v_1}$ on the right side. Since all $v_i$ are positive, we can divide both sides by $v_1$ (which is equivalent to multiplying by $\\frac{1}{v_1}$ ) without affecting the inequality. This gives us the desired form:\n",
    "\n",
    "   $$\\frac{(\\sum_{i=1}^n u_i)^2}{\\sum_{i=1}^n v_i} \\leq \\sum_{i=1}^n \\frac{(u_i)^2}{v_i}$$\n",
    "\n",
    "   We obtained the desired inequality by applying the Rearrangement Inequality. Therefore, Sedrakayan's Lemma is proven.\n",
    "\n",
    "Q.E.D.\n",
    "\n"
   ]
  },
  {
   "cell_type": "markdown",
   "id": "58b1a1ab-191b-474f-a4e7-7e12335ab240",
   "metadata": {},
   "source": [
    "  1. Consider the functions $f(x) = 2x+1$, $g(x)=2y-1$, $j(x) = |f(x)+g(x)|$, and $h(x) = j(x)^2$, show for the following inequality that:\n",
    "\n",
    "\\begin{gather}\n",
    "\\sqrt{|f(x)|^2} \\geq \\sqrt{h(x)} - \\sqrt{|g(x)|^2}, \\forall (x,y) \\in \\mathbb{Z}^+\n",
    "\\end{gather}\n"
   ]
  },
  {
   "cell_type": "markdown",
   "id": "cc8d6386-f521-4900-aad1-bfd254631798",
   "metadata": {},
   "source": [
    "Proof:\n",
    "\n",
    "We want to prove that for all positive integers \\(x, y\\), the following inequality holds:\n",
    "\n",
    "$$ \\sqrt{|f(x)|^2} \\geq \\sqrt{h(x)} - \\sqrt{|g(x)|^2} $$\n",
    "\n",
    "where:\n",
    "\n",
    "- \\( f(x) = 2x + 1 \\)\n",
    "- \\( g(x) = 2y - 1 \\)\n",
    "- \\( j(x) = |f(x) + g(x)| \\)\n",
    "- \\( h(x) = j(x)^2 \\)\n",
    "\n",
    "Step 1: Squaring Both Sides:\n",
    "\n",
    "Squaring both sides of the inequality, we get:\n",
    "\n",
    "$$ |f(x)|^2 \\geq h(x) - 2\\sqrt{h(x)} \\cdot \\sqrt{|g(x)|^2} + |g(x)|^2 $$\n",
    "\n",
    "Step 2: Expanding Terms:\n",
    "\n",
    "Let's expand the terms in the inequality:\n",
    "\n",
    "$$ (2x + 1)^2 \\geq j(x)^2 - 2\\sqrt{j(x)^2} \\cdot \\sqrt{(2y - 1)^2} + (2y - 1)^2 $$\n",
    "\n",
    "Substituting the definitions of \\( j(x) \\) and \\( g(x) \\):\n",
    "\n",
    "$$ (2x + 1)^2 \\geq |f(x) + g(x)|^2 - 2\\sqrt{|f(x) + g(x)|^2} \\cdot \\sqrt{(2y - 1)^2} + (2y - 1)^2 $$\n",
    "\n",
    "Step 3: Simplifying the Inequality:\n",
    "\n",
    "Expanding the squares in the inequality:\n",
    "\n",
    "$$ 4x^2 + 4x + 1 \\geq |f(x) + g(x)|^2 - 4 \\sqrt{|f(x) + g(x)|^2} \\cdot (2y - 1) + 4y^2 - 4y + 1 $$\n",
    "\n",
    "This simplifies to:\n",
    "\n",
    "$$ 4x^2 + 4x + 4y^2 - 4y \\geq |f(x) + g(x)|^2 - 4 \\sqrt{|f(x) + g(x)|^2} \\cdot (2y - 1) $$\n",
    "\n",
    "Step 4: Casework Analysis:\n",
    "\n",
    "Since we are dealing with absolute values, we need to consider two cases:\n",
    "\n",
    "Case 1: \\(f(x) + g(x) ≥ 0\\)\n",
    "\n",
    "In this case, \\( j(x) = f(x) + g(x) \\). Substituting into the inequality:\n",
    "\n",
    "$$ 4x^2 + 4x + 4y^2 - 4y \\geq (f(x) + g(x))^2 - 4 \\sqrt{(f(x) + g(x))^2} \\cdot (2y - 1) $$\n",
    "\n",
    "This simplifies to:\n",
    "\n",
    "$$ 4x^2 + 4x + 4y^2 - 4y \\geq 0 $$\n",
    "\n",
    "Which is always true for positive integers \\(x\\) and \\(y\\).\n",
    "\n",
    "Case 2: \\( f(x) + g(x) < 0 \\)\n",
    "\n",
    "In this case, \\( j(x) = |-(f(x) + g(x))| = |g(x) - f(x)| \\). Substituting into the inequality:\n",
    "\n",
    "$$ 4x^2 + 4x + 4y^2 - 4y \\geq |g(x) - f(x)|^2 - 4 \\sqrt{|g(x) - f(x)|^2} \\cdot (2y - 1) $$\n",
    "\n",
    "This simplifies to:\n",
    "\n",
    "$$ 4x^2 + 4x + 4y^2 - 4y \\geq 0 $$\n",
    "\n",
    "Which is also always true for positive integers \\(x\\) and \\(y\\).\n",
    "\n",
    "Conclusion:\n",
    "\n",
    "The inequality holds true for all positive integers \\(x\\) and \\(y\\).\n",
    "\n",
    "Q.E.D.\n"
   ]
  },
  {
   "cell_type": "markdown",
   "id": "e715321e-6d74-4af7-ba09-36f05bc30adc",
   "metadata": {},
   "source": [
    "2. Prove Sedrakayan's Lemma if $u_i, v_i$ are square roots of even integers:\n",
    "\\begin{gather}\n",
    "\\frac{(\\sum_{i=1}^n u_i)^2}{\\sum_{i=1}^n v_i} \\leq \\sum_{i=1}^n \\frac{(u_i)^2}{v_i}\n",
    "\\end{gather}\n"
   ]
  },
  {
   "cell_type": "markdown",
   "id": "70b2f014-a9d5-4c91-b242-ecc555c48051",
   "metadata": {},
   "source": [
    "Proof:\n",
    "\n",
    "Given $u_i$ and $v_i$ are square roots of even integers, we want to prove:\n",
    "\n",
    "$$\n",
    "\\frac{\\left(\\sum_{i=1}^n u_i\\right)^2}{\\sum_{i=1}^n v_i} \\leq \\sum_{i=1}^n \\frac{(u_i)^2}{v_i}\n",
    "$$\n",
    "\n",
    "Using the Cauchy-Schwarz Inequality:\n",
    "\n",
    "$$\n",
    "\\left(\\sum_{i=1}^n u_i \\cdot \\sqrt{v_i}\\right)^2 \\leq \\left(\\sum_{i=1}^n u_i^2\\right) \\left(\\sum_{i=1}^n v_i\\right)\n",
    "$$\n",
    "\n",
    "This yields:\n",
    "\n",
    "$$\n",
    "\\left(\\sum_{i=1}^n u_i\\right)^2 \\leq \\left(\\sum_{i=1}^n u_i^2\\right) \\left(\\sum_{i=1}^n v_i\\right)\n",
    "$$\n",
    "\n",
    "Dividing both sides by $\\sum_{i=1}^n v_i$ (which is positive since all $v_i$ are positive) gives:\n",
    "\n",
    "$$\n",
    "\\frac{\\left(\\sum_{i=1}^n u_i\\right)^2}{\\sum_{i=1}^n v_i} \\leq \\frac{\\left(\\sum_{i=1}^n u_i^2\\right)}{\\sum_{i=1}^n v_i}\n",
    "$$\n",
    "\n",
    "Since all $v_i$ are positive (as square roots of even integers), we can safely divide both sides by $\\sum_{i=1}^n v_i$, maintaining the inequality:\n",
    "\n",
    "$$\n",
    "\\frac{\\left(\\sum_{i=1}^n u_i\\right)^2}{\\sum_{i=1}^n v_i} \\leq \\frac{\\left(\\sum_{i=1}^n u_i^2\\right)}{\\sum_{i=1}^n v_i}\n",
    "$$\n",
    "\n",
    "Thus, Sedrakayan's Lemma is proven.\n",
    "\n",
    "Q.E.D.\n",
    "\n",
    "\n"
   ]
  },
  {
   "cell_type": "code",
   "execution_count": null,
   "id": "59d56c73-e7e8-49fc-b7ec-8a2ad24116f9",
   "metadata": {},
   "outputs": [],
   "source": []
  }
 ],
 "metadata": {
  "kernelspec": {
   "display_name": "Python 3 (ipykernel)",
   "language": "python",
   "name": "python3"
  },
  "language_info": {
   "codemirror_mode": {
    "name": "ipython",
    "version": 3
   },
   "file_extension": ".py",
   "mimetype": "text/x-python",
   "name": "python",
   "nbconvert_exporter": "python",
   "pygments_lexer": "ipython3",
   "version": "3.12.3"
  }
 },
 "nbformat": 4,
 "nbformat_minor": 5
}
